theories/proofmode/contiguous.v
@@ -331,10 +331,10 @@ Proof.
   naive_solver.
 Qed.
 
-Lemma isCorrectPC_range_perm_non_IE p b e a0 an :
+Lemma isCorrectPC_range_perm_non_IEpair p b e a0 an :
   isCorrectPC_range p b e a0 an →
   (a0 < an)%a →
-  p ≠ IE.
+  p ≠ IEpair.
 Proof.
   intros HH1 HH2. pose proof (isCorrectPC_range_perm _ _ _ _ _ HH1 HH2).
   naive_solver.
