theories/proofmode/proofmode_instr_rules.v
@@ -93,7 +93,7 @@ Ltac dispatch_instr_rule instr cont :=
              lazymatch w with
              (* TODO would also need more rules to differentiate all kind of equalities
              between addresses *)
-             | WCap IE _ _ _ =>
+             | WCap IEpair _ _ _ =>
               fail "No handled yet"
                  (* cont (wp_jnz_success_jmp_IE) *)
              | _ => cont (@wp_jnz_success_jmp)
@@ -107,7 +107,7 @@ Ltac dispatch_instr_rule instr cont :=
       lazymatch goal with
         | |- context [ environments.Esnoc _ _ (r ↦ᵣ ?w)%I ] =>
           lazymatch w with
-          | WCap IE _ _ _ =>
+          | WCap IEpair _ _ _ =>
               fail "No handled yet"
               (* cont (@wp_jmp_success_IE) *)
           (* TODO would also need more rules to differentiate all kind of equalities
@@ -122,7 +122,7 @@ Ltac dispatch_instr_rule instr cont :=
       lazymatch goal with
         | |- context [ environments.Esnoc _ _ (r ↦ᵣ ?w)%I ] =>
           lazymatch w with
-          | WCap IE _ _ _ => cont (@wp_jmp_success_IEpair)
+          | WCap IEpair _ _ _ => cont (@wp_jmp_success_IEpair)
           (* TODO would also need more rules to differentiate all kind of equalities
              between addresses *)
           | _ => cont (@wp_jmp_success)
